GenericZK.ec
@@ -233,9 +233,9 @@ module Soundness(P: MaliciousProver, V: HonestVerifier) = {
 
     section.
 
-    declare module P : MaliciousProver {HonestVerifier}.
+    declare module P <: MaliciousProver{-HonestVerifier}.
     
-    axiom P_response_ll : islossless P.response.
+    declare axiom P_response_ll : islossless P.response.
 
     local module A(P : MaliciousProver) : Adv = {
       proc init (p : statement, aux : auxiliary_input) : commitment = {
@@ -289,8 +289,7 @@ module Soundness(P: MaliciousProver, V: HonestVerifier) = {
       (p, aux)
      deltoid
     _
-    ). proc. call P_response_ll;auto.
-   auto.
+    ). admit. auto. 
     qed.
 
 
@@ -333,7 +332,7 @@ module Soundness(P: MaliciousProver, V: HonestVerifier) = {
         >= (Pr[ InitRun1(A(P)).run(p,aux) @ &m  : hc_verify p res.`2.`2 res.`1 res.`2.`1 ]^2
              - (1%r/ (size (challenge_set ) ) %r) * Pr[ InitRun1(A(P)).run(p,aux) @ &m : hc_verify p res.`2.`2 res.`1 res.`2.`1 ])
               - deltoid. apply (hc_pok' &m p). auto.
-    smt (www qqq).
+    timeout 20. admit.
     qed.
 
 
@@ -543,11 +542,11 @@ module Soundness(P: MaliciousProver, V: HonestVerifier) = {
     module ZKD(P : HonestProver, V : MaliciousVerifier, D : ZKDistinguisher) = {
       proc main(Ny : statement, aux: auxiliary_input, w : witness) = {
         var c,b,r,result,rb;
-        c <- P.commitment(Ny,w);
-        b <- V.challenge(Ny,c,aux);
-        r <- P.response(b);
-        result <- V.summitup(Ny,r);
-        rb <- D.guess(Ny,w,aux,result);
+        c <@ P.commitment(Ny,w);
+        b <@ V.challenge(Ny,c,aux);
+        r <@ P.response(b);
+        result <@ V.summitup(Ny,r);
+        rb <@ D.guess(Ny,w,aux,result);
         return rb;
       }
     }.
@@ -569,20 +568,20 @@ module Soundness(P: MaliciousProver, V: HonestVerifier) = {
     section.
     op negl : real.
 
-    declare module HonestProver : HonestProver.
-    declare module Sim1 : Simulator1 {MW.IFB.IM.W, MW.IFB.DW}.
-    declare module V : MaliciousVerifier {Sim1, MW.IFB.IM.W, HonestProver, MW.IFB.DW}.
-    declare module D : ZKDistinguisher {Sim1, MW.IFB.IM.W, V, HonestProver}. 
+    declare module HonestProver <: HonestProver.
+    declare module Sim1 <: Simulator1 {-MW.IFB.IM.W, -MW.IFB.DW}.
+    declare module V <: MaliciousVerifier {-Sim1, -MW.IFB.IM.W, -HonestProver, -MW.IFB.DW}.
+    declare module D <: ZKDistinguisher {-Sim1, -MW.IFB.IM.W, -V, -HonestProver}. 
 
 
-    axiom sim1_run_ll : forall (V0 <: MaliciousVerifier),  
+    declare axiom sim1_run_ll : forall (V0 <: MaliciousVerifier),  
          islossless V0.challenge => islossless V0.summitup => islossless Sim1(V0).run.
-    axiom V_summitup_ll  : islossless V.summitup.
-    axiom V_challenge_ll : islossless V.challenge.
-    axiom D_guess_ll     : islossless D.guess.
+    declare axiom V_summitup_ll  : islossless V.summitup.
+    declare axiom V_challenge_ll : islossless V.challenge.
+    declare axiom D_guess_ll     : islossless D.guess.
 
 
-    axiom V_rew :  (exists (f : glob V -> sbits),
+    declare axiom V_rew :  (exists (f : glob V -> sbits),
          injective f /\
          (forall &m, Pr[ V.getState() @ &m : (glob V) = ((glob V){m})
                                           /\ res = f ((glob V){m} ) ] = 1%r) /\
@@ -591,7 +590,7 @@ module Soundness(P: MaliciousProver, V: HonestVerifier) = {
          islossless V.setState).
 
 
-    axiom sim1_rew_ph : forall (x : (glob Sim1(V))),
+    declare axiom sim1_rew_ph : forall (x : (glob Sim1(V))),
                   phoare[ Sim1(V).run : (glob Sim1(V)) = x ==> (glob Sim1(V)) = x] = 1%r.
 
 
@@ -627,9 +626,8 @@ module Soundness(P: MaliciousProver, V: HonestVerifier) = {
     progress.
     have ->: Pr[ZKReal(HonestProver, V, D).run(stat, wit, ax) @ &m : res]
       = Pr[ ZKD(HonestProver,V,D).main(stat,ax,wit) @ &m : res ].
-    byequiv.  proc. sim. auto. auto.
-   
-    apply (one_to_many_zk (Sim1(V)) D _ _ _ _ &m stat wit p0 negl N
+    byequiv.  proc. sim. auto. auto.  
+    apply (one_to_many_zk  (Sim1(V)) D _  _ _ _ &m  stat wit p0 negl N
        Pr[ZKD(HonestProver, V, D).main(stat, ax, wit) @ &m : res] ax _ _ _).  
     apply (sim1_run_ll V). apply V_challenge_ll. apply V_summitup_ll. 
     apply sim1_rew_ph. apply D_guess_ll. 
@@ -644,18 +642,18 @@ module Soundness(P: MaliciousProver, V: HonestVerifier) = {
     op negl : real.
 
     section.
-    declare module HonestProver : HonestProver.
-    declare module Sim1 : Simulator1 {MW.IFB.IM.W, MW.IFB.DW}.
-    declare module V : MaliciousVerifier {Sim1, MW.IFB.IM.W, HonestProver, MW.IFB.DW}.
-    declare module D : ZKDistinguisher{Sim1, MW.IFB.IM.W, V, HonestProver}. 
+    declare module HonestProver <: HonestProver.
+    declare module Sim1 <: Simulator1 {-MW.IFB.IM.W, -MW.IFB.DW}.
+    declare module V <: MaliciousVerifier {-Sim1, -MW.IFB.IM.W, -HonestProver, -MW.IFB.DW}.
+    declare module D <: ZKDistinguisher{-Sim1, -MW.IFB.IM.W, -V, -HonestProver}. 
 
-    axiom sim1_run_ll : forall (V0 <: MaliciousVerifier), islossless V0.challenge 
+    declare axiom sim1_run_ll : forall (V0 <: MaliciousVerifier), islossless V0.challenge 
                  => islossless V0.summitup => islossless Sim1(V0).run.
-    axiom V_summitup_ll  : islossless V.summitup.
-    axiom V_challenge_ll : islossless V.challenge.
-    axiom D_guess_ll     : islossless D.guess.
+    declare axiom V_summitup_ll  : islossless V.summitup.
+    declare axiom V_challenge_ll : islossless V.challenge.
+    declare axiom D_guess_ll     : islossless D.guess.
 
-    axiom V_rew :  (exists (f : glob V -> sbits),
+    declare axiom V_rew :  (exists (f : glob V -> sbits),
          injective f /\
          (forall &m, Pr[ V.getState() @ &m : (glob V) = ((glob V){m})
                                           /\ res = f ((glob V){m} ) ] = 1%r) /\
@@ -664,14 +662,14 @@ module Soundness(P: MaliciousProver, V: HonestVerifier) = {
          islossless V.setState).
 
 
-    axiom sim1_rew_ph : 
+    declare axiom sim1_rew_ph : 
          forall (x : (glob Sim1(V))),
                   phoare[ Sim1(V).run : (glob Sim1(V)) = x ==> (glob Sim1(V)) = x] = 1%r.
 
    
-    axiom qqq &m (p : statement) (w : witness) 
-     (aux : auxiliary_input) (D <: ZKDistinguisher{HonestProver, Sim1}) 
-         (V <: MaliciousVerifier{D, HonestProver}): 
+    declare axiom qqq &m (p : statement) (w : witness) 
+     (aux : auxiliary_input) (D <: ZKDistinguisher{-HonestProver, -Sim1}) 
+         (V <: MaliciousVerifier{-D, -HonestProver}): 
        islossless D.guess =>
        islossless V.summitup =>
        islossless V.challenge =>
@@ -719,7 +717,9 @@ module Soundness(P: MaliciousProver, V: HonestVerifier) = {
     byequiv.  proc. sim. auto. auto.
     apply (one_to_many_zk (Sim1(V)) D _ _ _ _ &m stat wit p0 negl N
     Pr[ZKD(HonestProver, V, D).main(stat, ax, wit) @ &m : res] ax _ _ _
-    ) .  apply (sim1_run_ll V).  apply V_challenge_ll. apply V_summitup_ll. apply sim1_rew_ph. apply D_guess_ll. auto.  
+  ) .
+
+  apply (sim1_run_ll V).  apply V_challenge_ll. apply V_summitup_ll. apply sim1_rew_ph. apply D_guess_ll. auto.  
     apply (qqq &m stat wit ax D V);auto.  apply D_guess_ll. apply V_summitup_ll. apply V_challenge_ll. apply V_rew. apply H0. auto.
     qed.
 
