HC/PoK_Soundness.ec
@@ -1,5 +1,5 @@
 pragma Goals:printall.
-require import AllCore DBool Bool List Distr Int Aux DJoin.
+require import AllCore DBool Bool List Distr Int Aux DJoin RealExp.
 require import Aux Permutation Basics.
 
 require import SpecialSoundness.
@@ -9,9 +9,9 @@ clone import ComputationalPoK with op special_soundness_extract <- special_sound
 
 
 section.
-declare module P : MaliciousProver {HonestVerifier}.
+declare module P <: MaliciousProver {-HonestVerifier}.
 
-axiom P_response_ll : islossless P.response.
+declare axiom P_response_ll : islossless P.response.
 op ss : hc_prob.
 op auxx : auxiliary_input.
 
@@ -23,19 +23,18 @@ lemma hc_computational_PoK &m :
    (Pr[Soundness(P, HonestVerifier).run(ss, auxx) @ &m : res]^2
    - (1%r/2%r) * Pr[Soundness(P, HonestVerifier).run(ss, auxx) @ &m : res])
      - Pr[BindingExperiment(SpecialSoundnessBinder(SpecialSoundnessAdversary(P))).main() @ &m : res].
-apply (computational_PoK P  _ &m). apply P_response_ll.
+apply (computational_PoK P _ &m).  apply P_response_ll.
 apply (computational_special_soundness_binding (SpecialSoundnessAdversary(P)) &m).
 qed.
 
 
-require import RealExp.
+
 lemma hc_computational_soundness &m :
     ! in_language (fun x y => IsHC (x,y)) ss =>
      Pr[Soundness(P, HonestVerifier).run(ss, auxx) @ &m : res]
      <= sqrt (Pr[BindingExperiment(SpecialSoundnessBinder(SpecialSoundnessAdversary(P))).main() @ &m : res] + 1%r/2%r).
 proof.  progress.
-apply (computational_soundness P  _ &m ss auxx _ ). apply P_response_ll.
-auto.
+apply (computational_soundness P _ &m ss auxx _ );auto.  apply P_response_ll.
 apply (computational_special_soundness_binding (SpecialSoundnessAdversary(P)) &m).
 qed.
 
