HC/ZK.ec
@@ -2,6 +2,7 @@ pragma Goals:printall.
 require import AllCore DBool Bool List Distr Int Aux DJoin.
 
 require import Permutation Basics Sim1Property.
+
 import DJMM.
 import Sim1Property.ZK.
 
@@ -17,18 +18,18 @@ clone import RewBasics as Rew with type sbits <- sbits.
 
 section.
 
-declare module V : MaliciousVerifier{HonestProver, OMZK.MW.IFB.IM.W, OMZK.MW.IFB.DW}.
-declare module D : ZKDistinguisher{HonestProver, OMZK.MW.IFB.IM.W, V}.
+declare module V <: MaliciousVerifier{-HonestProver, -OMZK.MW.IFB.IM.W, -OMZK.MW.IFB.DW}.
+declare module D <: ZKDistinguisher{-HonestProver, -OMZK.MW.IFB.IM.W, -V}.
 
 
-axiom Sim1_run_ll : forall (V0 <: MaliciousVerifier), islossless V0.challenge => islossless V0.summitup => islossless Sim1(V0).run.
+declare axiom Sim1_run_ll : forall (V0 <: MaliciousVerifier), islossless V0.challenge => islossless V0.summitup => islossless Sim1(V0).run.
 
-axiom V_summitup_ll : islossless V.summitup. 
-axiom V_challenge_ll : islossless V.challenge.
-axiom D_guess_ll : islossless D.guess.
+declare axiom V_summitup_ll : islossless V.summitup. 
+declare axiom V_challenge_ll : islossless V.challenge.
+declare axiom D_guess_ll : islossless D.guess.
 
 
-axiom rewindable_V_plus : 
+declare axiom rewindable_V_plus :
         (exists (f : glob V -> sbits),
          injective f /\
          (forall &m, Pr[ V.getState() @ &m : (glob V) = ((glob V){m})
@@ -36,7 +37,6 @@ axiom rewindable_V_plus :
          (forall &m b (x: glob V), b = f x =>
            Pr[V.setState(b) @ &m : glob V = x] = 1%r) /\
          islossless V.setState).
-
 
 
 lemma hc_statistical_zk stat wit ax N &m:
@@ -50,13 +50,14 @@ progress.
 apply (statistical_zk HonestProver Sim1  V D _ _ _ _ _ _ _ stat wit ax N
   (inv 2%r - negl2) &m). apply Sim1_run_ll. apply V_summitup_ll. apply V_challenge_ll. apply D_guess_ll.
 apply rewindable_V_plus.
-apply (sim1_rew_ph V ). apply V_summitup_ll. apply V_challenge_ll. 
+apply (sim1_rew_ph V ). apply V_summitup_ll. apply V_challenge_ll.
 apply (rewindable_A_plus V). apply rewindable_V_plus.
 progress.
-apply (sim1_prop V D _ _  _ _ _ &m0 p w aux _ ).  apply (rewindable_A_plus V). exists f. split. auto. auto.
-auto. auto.   auto. apply negl2_prop. auto. auto. auto.
-apply (sim1assc V D);auto. apply (rewindable_A_plus V). apply rewindable_V_plus. apply D_guess_ll. apply V_summitup_ll.
-apply V_challenge_ll. apply negl2_prop. smt.
+apply (sim1_prop V D  _ _  _ _ _  &m0 p w aux _ );auto.  apply (rewindable_A_plus V). exists f. split. auto. auto.
+apply negl2_prop. auto. auto. auto.
+apply (sim1assc V D _ _ _ _ _ &m);auto.  apply (rewindable_A_plus V). apply rewindable_V_plus. apply D_guess_ll. apply V_summitup_ll.
+apply V_challenge_ll. apply negl2_prop. smt. 
 qed.
+
 
 end section.
