QR/PoK.ec
@@ -9,15 +9,16 @@ clone import ComputationalPoK with op special_soundness_extract <- special_sound
 
 
 section.
-declare module P : MaliciousProver {HonestVerifier}.
+declare module P <: MaliciousProver {-HonestVerifier}.
 
-axiom P_response_ll : islossless P.response.
+declare axiom P_response_ll : islossless P.response.
 
 lemma qr_computational_PoK &m  s aux: 
   Pr[Extractor(P).extract(s, aux) @ &m : IsSqRoot s res /\ unit s] >=
    (Pr[Soundness(P, HonestVerifier).run(s, aux) @ &m : res]^2
      - (1%r/2%r) * Pr[Soundness(P, HonestVerifier).run(s, aux) @ &m : res]).
-apply (statistical_PoK P  _ &m). apply P_response_ll.
+
+apply (statistical_PoK P  _ &m).  apply P_response_ll. 
 smt (perfect_special_soundness).
 qed.
 
